FoC/Computability/Compiler/Core/EncodedRewriters/ClosedConfigRunner/Projection/Padded/TailCleanup/PostPaddingCloseout.lean
@@ -1,4 +1,4 @@
-import FoC.Computability.Compiler.Core.EncodedRewriters.ClosedConfigRunner.Projection.Padded.TailCleanup.PostPaddingScratchExtender
+import FoC.Computability.Compiler.Core.EncodedRewriters.ClosedConfigRunner.Projection.Padded.TailCleanup.ScratchExt
 
 set_option doc.verso true
 
