FoC/Computability/Compiler/Core/EncodedRewriters/ClosedConfigRunner/Projection/Padded/TailCleanup/PostPaddingConstruction.lean
@@ -1,5 +1,5 @@
-import FoC.Computability.Compiler.Core.EncodedRewriters.ClosedConfigRunner.Projection.Padded.TailCleanup.PostPaddingConstruction.Core
-import FoC.Computability.Compiler.Core.EncodedRewriters.ClosedConfigRunner.Projection.Padded.TailCleanup.PostPaddingConstruction.PrefixErase
+import FoC.Computability.Compiler.Core.EncodedRewriters.ClosedConfigRunner.Projection.Padded.TailCleanup.PostPadCore
+import FoC.Computability.Compiler.Core.EncodedRewriters.ClosedConfigRunner.Projection.Padded.TailCleanup.PostPadPrefixErase
 
 set_option doc.verso true
 
