FoC/Computability/Compiler/Core/EncodedRewriters/ClosedConfigRunner/Projection/Quoter/SourceRestFinishCore/Final.lean
@@ -1,5 +1,5 @@
-import FoC.Computability.Compiler.Core.EncodedRewriters.ClosedConfigRunner.Projection.Quoter.SourceRestFinishCore.LiveTail.EmitterConstruction
-import FoC.Computability.Compiler.Core.EncodedRewriters.ClosedConfigRunner.Projection.Quoter.SourceRestFinishCore.LiveTail.JoinerConstruction
+import FoC.Computability.Compiler.Core.EncodedRewriters.ClosedConfigRunner.Projection.Quoter.SourceRestFinishCore.LTEmitterConstruction
+import FoC.Computability.Compiler.Core.EncodedRewriters.ClosedConfigRunner.Projection.Quoter.SourceRestFinishCore.LTJoinerConstruction
 
 set_option doc.verso true
 
