FoC/Computability/Compiler/Core/EncodedRewriters/ClosedConfigRunner/Projection/Quoter/SourceRestFinishCore/LiveTail.lean
@@ -1,6 +1,6 @@
-import FoC.Computability.Compiler.Core.EncodedRewriters.ClosedConfigRunner.Projection.Quoter.SourceRestFinishCore.LiveTail.EmitterRuns
-import FoC.Computability.Compiler.Core.EncodedRewriters.ClosedConfigRunner.Projection.Quoter.SourceRestFinishCore.LiveTail.JoinerStructured
-import FoC.Computability.Compiler.Core.EncodedRewriters.ClosedConfigRunner.Projection.Quoter.SourceRestFinishCore.LiveTail.JoinerRuns
+import FoC.Computability.Compiler.Core.EncodedRewriters.ClosedConfigRunner.Projection.Quoter.SourceRestFinishCore.LTEmitterRuns
+import FoC.Computability.Compiler.Core.EncodedRewriters.ClosedConfigRunner.Projection.Quoter.SourceRestFinishCore.LTJoinerStructured
+import FoC.Computability.Compiler.Core.EncodedRewriters.ClosedConfigRunner.Projection.Quoter.SourceRestFinishCore.LTJoinerRuns
 
 set_option doc.verso true
 
